c_stubs/common_tcp_karamel_compat.h
@@ -1,7 +1,6 @@
 #ifndef COMMON_TCP_KARAMEL_COMPAT_H
 #define COMMON_TCP_KARAMEL_COMPAT_H
 
-#define COMMON_TCP_KARAMEL_FULL_DECLS
 #include "common_tcp_karamel.h"
 
 #endif
