calc_sample/impl/Calc.Server.Socket.fst
@@ -11,6 +11,7 @@ module U16 = FStar.UInt16
 module U8 = FStar.UInt8
 module Vec = Pulse.Lib.Vec
 module MR = Pulse.Lib.MonotonicGhostRef
+module R = Pulse.Lib.Reference
 
 module CalcCP = Calc.Server.CanonicalProtocol
 
@@ -18,14 +19,19 @@ open Calc.Log
 open Calc.Wire
 open Calc.Impl.Types
 
+inline_for_extraction
 fn free_server_state
   (srv:server_state)
-  (#log:erased calc_log)
 requires
-  server_exactly srv log **
-  pure (Vec.is_full_vec srv.stack /\ Vec.is_full_vec srv.size)
+  exists* log.
+    server_exactly srv log **
+    pure (Vec.is_full_vec srv.stack /\ Vec.is_full_vec srv.size)
 ensures emp
 {
+  with log.
+    assert (
+      server_exactly srv log **
+      pure (Vec.is_full_vec srv.stack /\ Vec.is_full_vec srv.size));
   unfold (server_exactly srv log);
   with stack_bytes size_seq. _;
   Vec.free srv.stack;
@@ -33,29 +39,28 @@ ensures emp
   drop_ (MR.pts_to srv.ghost_log #1.0R log)
 }
 
-fn rec run_connection_loop
+inline_for_extraction
+fn run_connection_loop
   (srv:server_state)
   (ch:TCP.channel)
   (req:Vec.vec U8.t)
   (resp:Vec.vec U8.t)
   (fuel:SZ.t)
-  (#received:erased TCP.bytes)
-  (#sent:erased TCP.bytes)
-  (#log:erased calc_log)
 requires
-  server_exactly srv log **
-  TCP.is_channel ch received sent **
-  Vec.pts_to req 'req_bytes **
-  Vec.pts_to resp 'resp_bytes **
-  pure (
-    Seq.length 'req_bytes == 5 /\
-    Seq.length 'resp_bytes == 5 /\
-    Vec.length req == 5 /\
-    Vec.length resp == 5 /\
-    Vec.is_full_vec req /\
-    Vec.is_full_vec resp /\
-    Vec.is_full_vec srv.stack /\
-    Vec.is_full_vec srv.size)
+  exists* received sent log req_bytes resp_bytes.
+    server_exactly srv log **
+    TCP.is_channel ch received sent **
+    Vec.pts_to req req_bytes **
+    Vec.pts_to resp resp_bytes **
+    pure (
+      Seq.length req_bytes == 5 /\
+      Seq.length resp_bytes == 5 /\
+      Vec.length req == 5 /\
+      Vec.length resp == 5 /\
+      Vec.is_full_vec req /\
+      Vec.is_full_vec resp /\
+      Vec.is_full_vec srv.stack /\
+      Vec.is_full_vec srv.size)
 ensures
   exists* (received1:Ghost.erased TCP.bytes)
           (sent1:Ghost.erased TCP.bytes)
@@ -75,79 +80,129 @@ ensures
       Vec.is_full_vec resp /\
       Vec.is_full_vec srv.stack /\
       Vec.is_full_vec srv.size)
-decreases (SZ.v fuel)
 {
-  if (fuel = 0sz) {
-    ()
-  } else {
-    assert (pure (0 < SZ.v fuel));
-    Vec.to_array_pts_to req;
-    let nread = TCP.read_full ch (Vec.vec_to_array req) 5sz;
-    with req_bytes_after chunk. _;
+      let mut remaining = fuel;
+      let mut running = true;
+      while (
+        let keep = R.read running;
+        let rem = R.read remaining;
+        keep && not (rem = 0sz)
+      )
+        invariant live remaining
+        invariant live running
+        invariant exists* received_loop sent_loop log_loop req_bytes_loop resp_bytes_loop.
+          server_exactly srv (Ghost.reveal log_loop) **
+          TCP.is_channel ch (Ghost.reveal received_loop) (Ghost.reveal sent_loop) **
+          Vec.pts_to req req_bytes_loop **
+          Vec.pts_to resp resp_bytes_loop **
+          pure (
+            Seq.length req_bytes_loop == 5 /\
+            Seq.length resp_bytes_loop == 5 /\
+            Vec.length req == 5 /\
+            Vec.length resp == 5 /\
+            Vec.is_full_vec req /\
+            Vec.is_full_vec resp /\
+            Vec.is_full_vec srv.stack /\
+            Vec.is_full_vec srv.size /\
+            SZ.v (R.read remaining) <= SZ.v fuel)
+      {
+        with rem_live keep_live received_loop sent_loop log_loop req_bytes_loop resp_bytes_loop.
+          assert (
+            R.pts_to remaining rem_live **
+            R.pts_to running keep_live **
+            server_exactly srv (Ghost.reveal log_loop) **
+            TCP.is_channel ch (Ghost.reveal received_loop) (Ghost.reveal sent_loop) **
+            Vec.pts_to req req_bytes_loop **
+            Vec.pts_to resp resp_bytes_loop **
+            pure (
+              Seq.length req_bytes_loop == 5 /\
+              Seq.length resp_bytes_loop == 5 /\
+              Vec.length req == 5 /\
+              Vec.length resp == 5 /\
+              Vec.is_full_vec req /\
+              Vec.is_full_vec resp /\
+              Vec.is_full_vec srv.stack /\
+              Vec.is_full_vec srv.size /\
+              SZ.v rem_live <= SZ.v fuel));
+        Vec.to_array_pts_to req;
+        let nread = TCP.read_full ch (Vec.vec_to_array req) 5sz;
+        with req_bytes_after chunk. _;
     assert (pure (nread == 5sz));
     assert (pure (Seq.length req_bytes_after == 5));
     assert (pure (Seq.length chunk == 5));
     Vec.to_vec_pts_to req;
-    let tag = Calc.Impl.Parser.parse_tag req;
-    if U8.lt tag 6uy {
-      assert (pure (U8.v tag < 6));
-      assert (pure (tag == Seq.index req_bytes_after 0));
-      assert (pure (U8.v (Seq.index req_bytes_after 0) < 6));
-      CalcCP.lemma_parse_request_some_if_valid_tag req_bytes_after;
-      assert (pure (parse_request req_bytes_after <> None));
-      Calc.Server.process_request srv req resp;
-      with resp_bytes_after log_after. _;
-      Vec.pts_to_len resp;
-      assert (pure (Seq.length resp_bytes_after == 5));
-      Vec.to_array_pts_to resp;
-      let nwritten = TCP.write ch (Vec.vec_to_array resp) 5sz;
-      assert (pure (nwritten == 5sz));
-      Vec.to_vec_pts_to resp;
-      let received_after = Ghost.hide (Seq.append (Ghost.reveal received) chunk);
-      let sent_after =
-        Ghost.hide
-          (Seq.append
-            (Ghost.reveal sent)
+    if (nread = 5sz) {
+      let tag = Calc.Impl.Parser.parse_tag req;
+      if U8.lt tag 6uy {
+        assert (pure (U8.v tag < 6));
+        assert (pure (tag == Seq.index req_bytes_after 0));
+        assert (pure (U8.v (Seq.index req_bytes_after 0) < 6));
+        CalcCP.lemma_parse_request_some_if_valid_tag req_bytes_after;
+        assert (pure (parse_request req_bytes_after <> None));
+        Calc.Server.process_request srv req resp;
+        with resp_bytes_after log_after. _;
+        Vec.pts_to_len resp;
+        assert (pure (Seq.length resp_bytes_after == 5));
+        Vec.to_array_pts_to resp;
+        let nwritten = TCP.write ch (Vec.vec_to_array resp) 5sz;
+        assert (pure (nwritten == 5sz));
+        Vec.to_vec_pts_to resp;
+        let received_after = Ghost.hide (Seq.append (Ghost.reveal received_loop) chunk);
+        let sent_after =
+          Ghost.hide
+            (Seq.append
+              (Ghost.reveal sent_loop)
+              (if SZ.v nwritten <= Seq.length resp_bytes_after
+               then Seq.slice resp_bytes_after 0 (SZ.v nwritten)
+               else Seq.create 0 0uy));
+        assert (pure (Ghost.reveal received_after == Seq.append (Ghost.reveal received_loop) chunk));
+        assert (pure (Ghost.reveal sent_after ==
+          Seq.append
+            (Ghost.reveal sent_loop)
             (if SZ.v nwritten <= Seq.length resp_bytes_after
              then Seq.slice resp_bytes_after 0 (SZ.v nwritten)
-             else Seq.create 0 0uy));
-      assert (pure (Ghost.reveal received_after == Seq.append (Ghost.reveal received) chunk));
-      assert (pure (Ghost.reveal sent_after ==
-        Seq.append
-          (Ghost.reveal sent)
-          (if SZ.v nwritten <= Seq.length resp_bytes_after
-           then Seq.slice resp_bytes_after 0 (SZ.v nwritten)
-           else Seq.create 0 0uy)));
+             else Seq.create 0 0uy)));
+        rewrite
+          (TCP.is_channel
+            ch
+            (Seq.append (Ghost.reveal received_loop) chunk)
+            (Seq.append
+              (Ghost.reveal sent_loop)
+              (if SZ.v nwritten <= Seq.length resp_bytes_after
+               then Seq.slice resp_bytes_after 0 (SZ.v nwritten)
+               else Seq.create 0 0uy)))
+          as
+          (TCP.is_channel ch (Ghost.reveal received_after) (Ghost.reveal sent_after));
+        if (nwritten = 5sz) {
+          let rem_now = R.read remaining;
+          assert (pure (not (rem_now = 0sz)));
+          assert (pure (0 < SZ.v rem_now));
+          let next = SZ.sub rem_now 1sz;
+          assert (pure (SZ.v next < SZ.v rem_now));
+          assert (pure (SZ.v next <= SZ.v fuel));
+          remaining := next
+        } else {
+          running := false
+        }
+      } else {
+        let received_after = Ghost.hide (Seq.append (Ghost.reveal received_loop) chunk);
+        let sent_after = Ghost.hide (Ghost.reveal sent_loop);
+        assert (pure (Seq.length req_bytes_after == 5));
+        assert (pure (Seq.length resp_bytes_loop == 5));
+        rewrite
+          (TCP.is_channel ch (Seq.append (Ghost.reveal received_loop) chunk) (Ghost.reveal sent_loop))
+          as
+          (TCP.is_channel ch (Ghost.reveal received_after) (Ghost.reveal sent_after));
+        running := false
+      }
+    } else {
+      let received_after = Ghost.hide (Seq.append (Ghost.reveal received_loop) chunk);
+      let sent_after = Ghost.hide (Ghost.reveal sent_loop);
       rewrite
-        (TCP.is_channel
-          ch
-          (Seq.append (Ghost.reveal received) chunk)
-          (Seq.append
-            (Ghost.reveal sent)
-            (if SZ.v nwritten <= Seq.length resp_bytes_after
-             then Seq.slice resp_bytes_after 0 (SZ.v nwritten)
-             else Seq.create 0 0uy)))
+        (TCP.is_channel ch (Seq.append (Ghost.reveal received_loop) chunk) (Ghost.reveal sent_loop))
         as
         (TCP.is_channel ch (Ghost.reveal received_after) (Ghost.reveal sent_after));
-      let log_after_e = Ghost.hide log_after;
-      let next_fuel = SZ.sub fuel 1sz;
-      assert (pure (SZ.v next_fuel < SZ.v fuel));
-      run_connection_loop
-        srv
-        ch
-        req
-        resp
-        next_fuel
-        #received_after
-        #sent_after
-        #log_after_e
-    } else {
-      let received_after = Ghost.hide (Seq.append (Ghost.reveal received) chunk);
-      let sent_after = Ghost.hide (Ghost.reveal sent);
-      let log_after = Ghost.hide (Ghost.reveal log);
-      assert (pure (Seq.length req_bytes_after == 5));
-      assert (pure (Seq.length 'resp_bytes == 5));
-      ()
+      running := false
     }
   }
 }
@@ -166,10 +221,7 @@ ensures emp
     ch
     req
     resp
-    fuel
-    #(Seq.create 0 0uy)
-    #(Seq.create 0 0uy)
-    #initial_log;
+    fuel;
   with received1 sent1 log1 req_bytes1 resp_bytes1. _;
   TCP.close ch;
   Vec.free req;
@@ -208,10 +260,7 @@ ensures pts_to bind_host 'bind_host_bytes
             ch
             req
             resp
-            fuel
-            #(Seq.create 0 0uy)
-            #(Seq.create 0 0uy)
-            #initial_log;
+            fuel;
           with received1 sent1 log1 req_bytes1 resp_bytes1. _;
           TCP.close ch;
           Vec.free req;
